theories/OGS/Soundness.v
@@ -3,7 +3,7 @@ From Coinduction Require Import coinduction tactics.
 From OGS Require Import Prelude.
 From OGS.Utils Require Import Ctx Rel.
 From OGS.Game Require Import HalfGame Event.
-From OGS.OGS Require Import Subst Obs Machine Game Strategy CompGuarded Adequacy Congruence.
+From OGS.OGS Require Export Subst Obs Machine Game Strategy CompGuarded Adequacy Congruence.
 From OGS.ITree Require Import ITree Eq Delay Structure Properties Guarded.
 
 Open Scope ctx_scope.
